SystemF2Effect: generalise maskOnCap
Ignore-this: 3bea0ce4a685e347871e05c1a8359042

darcs-hash:20130211101306-08f32-8517c98058c1e7a4a6524a8080427d9034e3a070

devel/Iron/SystemF2Effect/Type/Operator/MaskOnCap.v
@@ -7,52 +7,51 @@ Require Import Iron.SystemF2Effect.Type.Exp.
 
 (* Mask effects on the given region, 
    replacing with the bottom effect. *)
-Fixpoint maskOnCap (r : nat) (e : ty) : ty
+Fixpoint maskOnCap (p : nat -> bool) (e : ty) : ty
  := match e with
     |  TVar tc       => TVar tc
-    |  TForall k t1  => TForall k (maskOnCap r t1)
-    |  TApp t1 t2    => TApp (maskOnCap r t1) (maskOnCap r t2)
-    |  TSum t1 t2    => TSum (maskOnCap r t1) (maskOnCap r t2)
+    |  TForall k t1  => TForall k (maskOnCap p t1)
+    |  TApp t1 t2    => TApp (maskOnCap p t1) (maskOnCap p t2)
+    |  TSum t1 t2    => TSum (maskOnCap p t1) (maskOnCap p t2)
     |  TBot k        => TBot k
 
     |  TCon0 tc      => TCon0 tc
 
     |  TCon1 tc t1
     => match t1 with
-       | TCap (TyCapRegion n') 
-       => if beq_nat r n' 
+       | TCap (TyCapRegion n) 
+       => if p n
              then TBot KEffect 
-             else TCon1 tc (maskOnCap r t1)
+             else TCon1 tc (maskOnCap p t1)
 
-       | _ =>     TCon1 tc (maskOnCap r t1)
+       | _ =>     TCon1 tc (maskOnCap p t1)
        end
     
-    | TCon2 tc t1 t2 => TCon2 tc (maskOnCap r t1) (maskOnCap r t2)
+    | TCon2 tc t1 t2 => TCon2 tc (maskOnCap p t1) (maskOnCap p t2)
 
     | TCap  tc       => TCap tc
     end.
-Arguments maskOnCap r e : simpl nomatch.
+Arguments maskOnCap p e : simpl nomatch.
 
 
 (********************************************************************)
 (* Helper Lemmas *)
 Lemma maskOnCap_TBot_cases
- :  forall d tc n
- ,  maskOnCap d (TCon1 tc (TCap (TyCapRegion n))) = TBot KEffect 
- -> d = n.
+ :  forall p tc n
+ ,  maskOnCap p (TCon1 tc (TCap (TyCapRegion n))) = TBot KEffect 
+ -> p n = true.
 Proof.
  intros.
  unfold maskOnCap in H.
- break (beq_nat d n).
-  norm_beq_nat. auto.
-  nope.
+ break (p n).
+  auto. nope.
 Qed.
 
 
 Lemma maskOnCap_TCon1_cases
- :   forall d tc t
- ,   maskOnCap d (TCon1 tc t) = TBot KEffect
- \/  maskOnCap d (TCon1 tc t) = TCon1 tc (maskOnCap d t).
+ :   forall p tc t
+ ,   maskOnCap p (TCon1 tc t) = TBot KEffect
+ \/  maskOnCap p (TCon1 tc t) = TCon1 tc (maskOnCap p t).
 Proof.
  intros. 
  destruct t; simpl; rip.
@@ -62,24 +61,29 @@ Qed.
 
 
 Lemma maskOnCap_nomatch
- : forall n tc t2
- ,  t2 <> TCap (TyCapRegion n)
- -> maskOnCap n (TCon1 tc t2)    = TCon1 tc (maskOnCap n t2).
+ : forall p tc t2
+ ,  (forall n, t2 = TCap (TyCapRegion n) -> p n = false)
+ -> maskOnCap p (TCon1 tc t2)    = TCon1 tc (maskOnCap p t2).
 Proof.
  intros.
  destruct t2; snorm.
  
  Case "TCap".
   unfold maskOnCap.
-  destruct t. norm. congruence.
+  destruct t.
+  break (p n).
+   spec H n. 
+    have (TCap (TyCapRegion n) = TCap (TyCapRegion n)).
+    rip. congruence.
+   auto.
 Qed.
 
 
 (********************************************************************)
 Lemma maskOnCap_kind
- :  forall ke sp t k n
+ :  forall ke sp t k p
  ,  KIND ke sp t k 
- -> KIND ke sp (maskOnCap n t) k.
+ -> KIND ke sp (maskOnCap p t) k.
 Proof.
  intros. gen ke sp k.
  induction t; intros; inverts_kind; simpl; auto.
@@ -95,18 +99,17 @@ Proof.
 
   SCase "TCap".
    destruct t0. 
-    unfold maskOnCap. split_if.
-
-     norm_beq_nat. subst. inverts_kind.
+    unfold maskOnCap. 
+    split_if.
      destruct t; simpl in *.
       inverts H4. auto.
       inverts H4. auto.
       inverts H4. auto.
 
-     norm_beq_nat. inverts_kind.
-     destruct t; simpl in *; inverts H4; eapply KiCon1; simpl; eauto.
+     destruct t; simpl in *;
+      inverts H4; eapply KiCon1; simpl; eauto.
 
- Case "TCap".
+ Case "TCon2".
   spec IHt1 H5.
   spec IHt2 H7.
   eapply KiCon2; eauto.
@@ -136,12 +139,12 @@ Qed.
 
 
 Lemma maskOnCap_substTT
- : forall n d t1 t2
- ,  t2 <> TCap (TyCapRegion n)
- -> maskOnCap n (substTT d t2 t1) 
- =  substTT d (maskOnCap n t2) (maskOnCap n t1).
+ : forall p d t1 t2
+ ,  (forall n, t2 = TCap (TyCapRegion n) -> p n = false)
+ -> maskOnCap p (substTT d t2 t1) 
+ =  substTT   d (maskOnCap p t2) (maskOnCap p t1).
 Proof. 
- intros. gen n d t2. 
+ intros. gen p d t2. 
  induction t1; intros;
   try (solve [snorm; f_equal; rewritess; auto]).
 
@@ -159,7 +162,7 @@ Proof.
    try (solve [snorm; f_equal; rip]).
 
    SCase "TVar".
-    lets D: substTT_TVar_cases d n0 t2.
+    lets D: substTT_TVar_cases d n t2.
     inverts D. 
 
     SSSCase "substTT matches".
@@ -178,13 +181,13 @@ Proof.
      norm; subst; omega.
 
    SCase "TCap".
-    lets D: maskOnCap_TCon1_cases n t (TCap t0).
+    lets D: maskOnCap_TCon1_cases p t (TCap t0).
     inverts D.
 
     SSCase "maskOnCap matches".
      destruct t0.
      rewritess.
-     lets D: maskOnCap_TBot_cases n t n0. 
+     lets D: maskOnCap_TBot_cases p t n. 
       rip.
 
     SSCase "maskOnCap doesn't match".
